matching-logic/src/Theories/Sorts.v
@@ -11,7 +11,7 @@ From Coq.Classes Require Import Morphisms_Prop.
 From stdpp Require Import base sets.
 
 From MatchingLogic Require Import Syntax Semantics DerivedOperators Utils.extralibrary.
-Require Import MatchingLogic.Theories.Definedness.
+Require Import MatchingLogic.Theories.Definedness_Semantics.
 
 Import MatchingLogic.Syntax.Notations.
 Import MatchingLogic.Syntax.BoundVarSugar.
@@ -19,133 +19,10 @@ Import MatchingLogic.Semantics.Notations.
 Import MatchingLogic.IndexManipulation.
 Import MatchingLogic.DerivedOperators.Notations.
 
-
-Inductive Symbols := inhabitant.
-
-Instance Symbols_eqdec : EqDecision Symbols.
-Proof. unfold EqDecision. intros x y. unfold Decision. destruct x. decide equality. (*solve_decision.*) Defined.
-
-Section sorts.
-
-  Context {Σ : Signature}.
-
-  Class Syntax :=
-    { inj : Symbols -> symbols;
-      imported_definedness :> Definedness.Syntax;
-    }.
-
-  Context {self : Syntax}.
-
-  Local Definition sym (s : Symbols) : Pattern :=
-    patt_sym (inj s).
-  
-  Example test_pattern_1 := patt_equal (sym inhabitant) (sym inhabitant).
-  Definition patt_inhabitant_set(phi : Pattern) : Pattern := sym inhabitant $ phi.
-
-
-  Lemma bevar_subst_inhabitant_set ψ (wfcψ : well_formed_closed ψ) x ϕ :
-    bevar_subst (patt_inhabitant_set ϕ) ψ x = patt_inhabitant_set (bevar_subst ϕ ψ x).
-  Proof. unfold patt_inhabitant_set. simpl_bevar_subst. reflexivity. Qed.
-  
-  Lemma bsvar_subst_inhabitant_set ψ (wfcψ : well_formed_closed ψ) x ϕ :
-    bsvar_subst (patt_inhabitant_set ϕ) ψ x = patt_inhabitant_set (bsvar_subst ϕ ψ x).
-  Proof. unfold patt_inhabitant_set. simpl_bsvar_subst. reflexivity. Qed.
-  
-  #[global]
-   Instance Unary_inhabitant_set : Unary patt_inhabitant_set :=
-    {| unary_bevar_subst := bevar_subst_inhabitant_set ;
-       unary_bsvar_subst := bsvar_subst_inhabitant_set ;
-    |}.
-
-  Definition patt_forall_of_sort (sort phi : Pattern) : Pattern :=
-    patt_forall ((patt_in (patt_bound_evar 0) (patt_inhabitant_set (nest_ex sort))) ---> phi).
-
-  Definition patt_exists_of_sort (sort phi : Pattern) : Pattern :=
-    patt_exists ((patt_in (patt_bound_evar 0) (patt_inhabitant_set (nest_ex sort))) and phi).
-
-  Lemma bevar_subst_forall_of_sort s ψ (wfcψ : well_formed_closed ψ) db ϕ :
-    bevar_subst (patt_forall_of_sort s ϕ) ψ db = patt_forall_of_sort (bevar_subst s ψ db) (bevar_subst ϕ ψ (S db)).
-  Proof.
-    unfold patt_forall_of_sort.
-    repeat (rewrite simpl_bevar_subst';[assumption|]).
-    simpl. unfold nest_ex. replace (S db) with (db + 1) by lia. rewrite nest_ex_gt; auto. lia.
-  Qed.
-
-  Lemma bsvar_subst_forall_of_sort s ψ (wfcψ : well_formed_closed ψ) db ϕ :
-    bsvar_subst (patt_forall_of_sort s ϕ) ψ db = patt_forall_of_sort (bsvar_subst s ψ db) (bsvar_subst ϕ ψ db).
-  Proof.
-    unfold patt_forall_of_sort.
-    repeat (rewrite simpl_bsvar_subst';[assumption|]).
-    simpl.
-    rewrite bsvar_subst_nest_ex_aux_comm.
-    { unfold well_formed_closed in wfcψ. destruct_and!. assumption. }
-    reflexivity.
-  Qed.
-
-  Lemma bevar_subst_exists_of_sort s ψ (wfcψ : well_formed_closed ψ) db ϕ :
-    bevar_subst (patt_exists_of_sort s ϕ) ψ db = patt_exists_of_sort (bevar_subst s ψ db) (bevar_subst ϕ ψ (db+1)).
-  Proof.
-    unfold patt_exists_of_sort.
-    repeat (rewrite simpl_bevar_subst';[assumption|]).
-    (* TODO rewrite all _+1 to 1+_ *)
-    rewrite PeanoNat.Nat.add_comm. simpl.
-    unfold nest_ex.
-    simpl. unfold nest_ex. replace (S db) with (db + 1) by lia. rewrite nest_ex_gt; auto. lia.
-  Qed.
-
-  Lemma bsvar_subst_exists_of_sort s ψ (wfcψ : well_formed_closed ψ) db ϕ :
-    bsvar_subst (patt_exists_of_sort s ϕ) ψ db = patt_exists_of_sort (bsvar_subst s ψ db) (bsvar_subst ϕ ψ db).
-  Proof.
-    unfold patt_exists_of_sort.
-    repeat (rewrite simpl_bsvar_subst';[assumption|]).
-    simpl.
-    rewrite bsvar_subst_nest_ex_aux_comm.
-    { unfold well_formed_closed in wfcψ. destruct_and!. assumption. }
-    reflexivity.
-  Qed.
-    
-  #[global]
-   Instance EBinder_forall_of_sort s : EBinder (patt_forall_of_sort s) _ _:=
-    {|
-    ebinder_bevar_subst := bevar_subst_forall_of_sort s ;
-    ebinder_bsvar_subst := bsvar_subst_forall_of_sort s ;
-    |}.
-
-  #[global]
-   Instance EBinder_exists_of_sort s : EBinder (patt_exists_of_sort s) _ _:=
-    {|
-    ebinder_bevar_subst := bevar_subst_exists_of_sort s ;
-    ebinder_bsvar_subst := bsvar_subst_exists_of_sort s ;
-    |}.
-  
-  (* TODO patt_forall_of_sort and patt_exists_of_sorts are duals - a lemma *)
-
-  (* TODO a lemma about patt_forall_of_sort *)
-  
-  Definition patt_total_function(phi from to : Pattern) : Pattern :=
-    patt_forall_of_sort from (patt_exists_of_sort (nest_ex to) (patt_equal (patt_app (nest_ex (nest_ex phi)) b1) b0)).
-
-  Definition patt_partial_function(phi from to : Pattern) : Pattern :=
-    patt_forall_of_sort from (patt_exists_of_sort (nest_ex to) (patt_subseteq (patt_app (nest_ex (nest_ex phi)) b1) b0)).
-
-
-  (* Assuming `f` is a total function, says it is injective on given domain. Does not quite work for partial functions. *)
-  Definition patt_total_function_injective f from : Pattern :=
-    patt_forall_of_sort from (patt_forall_of_sort (nest_ex from) (patt_imp (patt_equal (patt_app (nest_ex (nest_ex f)) b1) (patt_app (nest_ex (nest_ex f)) b0)) (patt_equal b1 b0))).
-
-  (* Assuming `f` is a partial function, says it is injective on given domain. Works for total functions, too. *)
-  Definition patt_partial_function_injective f from : Pattern :=
-    patt_forall_of_sort
-      from
-      (patt_forall_of_sort
-         (nest_ex from)
-         (patt_imp
-            (patt_not (patt_equal (patt_app (nest_ex (nest_ex f)) b1) patt_bott ))
-            (patt_imp (patt_equal (patt_app (nest_ex (nest_ex f)) b1) (patt_app (nest_ex (nest_ex f)) b0)) (patt_equal b1 b0)))).
-  
-
   Section with_model.
-    Context {M : Model}.
+    Context
+      {Σ : Signature}
+      {M : Model}.
     Hypothesis M_satisfies_theory : M ⊨ᵀ Definedness.theory.
 
     Definition Mpatt_inhabitant_set m := app_ext (sym_interp M (inj inhabitant)) {[m]}.
