matching-logic/src/Theories/Definedness_Semantics.v
@@ -1,0 +1,30 @@
+From Coq Require Import ssreflect ssrfun ssrbool.
+Set Implicit Arguments.
+Unset Strict Implicit.
+Unset Printing Implicit Defensive.
+
+From Ltac2 Require Import Ltac2.
+
+Require Import Equations.Prop.Equations.
+
+From Coq Require Import String Ensembles Setoid.
+Require Import Coq.Program.Equality.
+Require Import Coq.Logic.Classical_Prop.
+From Coq.Logic Require Import FunctionalExtensionality Eqdep_dec.
+From Coq.Classes Require Import Morphisms_Prop.
+From Coq.Unicode Require Import Utf8.
+From Coq.micromega Require Import Lia.
+
+From MatchingLogic Require Import Syntax NamedAxioms Semantics DerivedOperators.
+From MatchingLogic.Utils Require Import stdpp_ext.
+
+From stdpp Require Import base fin_sets sets propset proof_irrel option list.
+
+Import extralibrary.
+
+Require Import MatchingLogic.Theories.Definedness_Syntax.
+
+Import MatchingLogic.Syntax.Notations.
+Import MatchingLogic.Semantics.Notations.
+Import MatchingLogic.DerivedOperators.Notations.
+Import MatchingLogic.Syntax.BoundVarSugar.
