matching-logic/src/Theories/Definedness_Syntax.v
@@ -1,0 +1,172 @@
+(* In this module we define the definedness symbol and use it to build derived notions
+   like totality and equality.
+ *)
+ From Coq Require Import ssreflect ssrfun ssrbool.
+ Set Implicit Arguments.
+ Unset Strict Implicit.
+ Unset Printing Implicit Defensive.
+  
+ From Coq Require Import String Setoid.
+ Require Import Coq.Program.Equality.
+ Require Import Coq.Logic.Classical_Prop.
+ From Coq.Logic Require Import FunctionalExtensionality Eqdep_dec.
+ From Coq.Classes Require Import Morphisms_Prop.
+ From Coq.Unicode Require Import Utf8.
+ From Coq.micromega Require Import Lia.
+ 
+ From MatchingLogic Require Import Syntax NamedAxioms DerivedOperators.
+ From MatchingLogic.Utils Require Import stdpp_ext.
+ 
+ From stdpp Require Import base fin_sets sets propset proof_irrel option list.
+ 
+ Import extralibrary.
+ 
+ Import MatchingLogic.Syntax.Notations.
+ Import MatchingLogic.DerivedOperators.Notations.
+ Import MatchingLogic.Syntax.BoundVarSugar.
+
+ Open Scope ml_scope.
+
+(* We have only one symbol *)
+Inductive Symbols := definedness.
+
+Instance Symbols_eqdec : EqDecision Symbols.
+Proof. unfold EqDecision. intros x y. unfold Decision. destruct x. decide equality. (*solve_decision.*) Defined.
+
+  Class Syntax {Σ : Signature} :=
+    {
+    (* 'Symbols' are a 'subset' of all the symbols from the Σnature *)
+    inj: Symbols -> symbols;
+    (* TODO make it injective? *)
+    (* for convenience *)
+    }.
+
+Section definedness.
+  
+  Context {Σ : Signature}.
+
+  Context {syntax : Syntax}.
+
+  Definition patt_defined (phi : Pattern) : Pattern :=
+    patt_sym (inj definedness) $ phi.
+  
+  Definition patt_total (phi: Pattern) : Pattern :=
+    patt_not (patt_defined (patt_not phi)).
+
+  Definition patt_subseteq (phi1 phi2 : Pattern) : Pattern :=
+    patt_total (phi1 ---> phi2).
+  
+  Definition patt_equal (phi1 phi2 : Pattern) : Pattern :=
+    patt_total (phi1 <---> phi2).
+
+  Definition patt_in (phi1 phi2 : Pattern) : Pattern :=
+    patt_defined (patt_and phi1 phi2).
+
+  Definition AC_patt_defined : Application_context :=
+    @ctx_app_r _ (patt_sym (inj definedness)) box ltac:(auto).
+
+  Definition is_predicate_pattern ψ : Pattern :=
+    (patt_equal ψ patt_top) or (patt_equal ψ patt_bott).
+End definedness.
+
+Module Notations.
+  Import Syntax.
+
+  Notation "⌈ p ⌉" := (patt_defined p) : ml_scope.
+  Notation "⌊ p ⌋" := (patt_total p) : ml_scope.
+  Notation "p =ml q" := (patt_equal p q) (at level 67) : ml_scope.
+  Notation "p ⊆ml q" := (patt_subseteq p q) (at level 67) : ml_scope.
+  Notation "p ∈ml q" := (patt_in p q) (at level 67) : ml_scope.
+  
+End Notations.
+
+Import Notations.
+
+Section definedness.
+  Context
+    {Σ : Signature}
+    {syntax : Syntax}
+  .
+
+  Lemma well_formed_defined ϕ:
+    well_formed ϕ = true ->
+    well_formed ⌈ ϕ ⌉ = true.
+  Proof.
+    intros Hwfϕ.
+    unfold patt_defined.
+    auto.
+  Qed.
+
+  #[local]
+   Hint Resolve well_formed_defined : core.
+
+  Lemma well_formed_total ϕ:
+    well_formed ϕ = true ->
+    well_formed ⌊ ϕ ⌋ = true.
+  Proof.
+    intros Hwfϕ.
+    unfold patt_total.
+    auto.
+  Qed.
+
+  #[local]
+   Hint Resolve well_formed_total : core.
+  
+  Lemma well_formed_equal (phi1 phi2 : Pattern) :
+    well_formed phi1 = true ->
+    well_formed phi2 = true ->
+    well_formed (phi1 =ml phi2) = true.
+  Proof.
+    intros wfphi1 wfphi2. unfold "=ml". auto.
+  Qed.
+
+  #[local]
+   Hint Resolve well_formed_equal : core.
+  
+  Lemma well_formed_subseteq (phi1 phi2 : Pattern) :
+    well_formed phi1 = true ->
+    well_formed phi2 = true ->
+    well_formed (phi1 ⊆ml phi2) = true.
+  Proof.
+    intros wfphi1 wfphi2. unfold "⊆ml". auto.
+  Qed.
+
+  #[local]
+   Hint Resolve well_formed_subseteq : core.
+
+  Lemma well_formed_in (phi1 phi2 : Pattern) :
+    well_formed phi1 = true ->
+    well_formed phi2 = true ->
+    well_formed (phi1 ∈ml phi2) = true.
+  Proof.
+    intros wfphi1 wfphi2. unfold "∈ml". auto.
+  Qed.
+
+  #[local]
+   Hint Resolve well_formed_in : core.
+
+  
+  Let sym (s : Symbols) : Pattern :=
+    @patt_sym Σ (inj s).
+
+  Definition ev_x := (evar_fresh []).
+  Definition p_x := patt_free_evar ev_x.
+  
+  Inductive AxiomName := AxDefinedness.
+
+  Definition axiom(name : AxiomName) : Pattern :=
+    match name with
+    | AxDefinedness => patt_defined p_x
+    end.
+
+  Program Definition named_axioms : NamedAxioms :=
+    {| NAName := AxiomName;
+      NAAxiom := axiom;
+    |}.
+  Next Obligation.
+    intros name. destruct name; simpl; wf_auto2.
+  Qed.
+
+  Definition theory := theory_of_NamedAxioms named_axioms.
+
+  End definedness.
